LambdaS5/coq/LjsAuxiliary.v
@@ -10,14 +10,8 @@ Definition object_binds st ptr obj :=
 Definition object_indom st ptr :=
     Heap.indom (object_heap st) ptr.
 
-Definition value_binds st loc v :=
-    Heap.binds (value_heap st) loc v.
-
-Definition value_indom st loc :=
-    Heap.indom (value_heap st) loc.
-
 Definition id_binds c i loc :=
-    Heap.binds (loc_heap c) i loc.
+    Heap.binds (value_heap c) i loc.
 
 Definition id_indom c i :=
-    Heap.indom (loc_heap c) i.
+    Heap.indom (value_heap c) i.
