LambdaS5/coq/LjsOperators.v
@@ -12,7 +12,6 @@ Implicit Type store : store.
 
 Implicit Type st : store.
 Implicit Type v : value.
-Implicit Type loc : value_loc.
 Implicit Type s : string.
 Implicit Type n : number.
 Implicit Type i : id.
@@ -38,7 +37,7 @@ Definition typeof store (v : value) :=
       | _ => result_some (value_string "function")
       end
     )
-  | value_closure _ _ _ _ => result_fail "typeof got lambda"
+  | value_closure _ => result_fail "typeof got lambda"
   end
 .
 
@@ -53,7 +52,7 @@ Definition is_primitive v :=
 
 Definition is_closure v :=
   match v with
-  | value_closure _ _ _ _ =>
+  | value_closure _ =>
     result_some value_true
   | _ =>
     result_some value_false
@@ -143,7 +142,7 @@ Definition nnot store (v : value) :=
   | value_string "" => result_some value_true
   | value_string _ => result_some value_false
   | value_object _ => result_some value_false
-  | value_closure _ _ _ _ => result_some value_false
+  | value_closure _ => result_some value_false
   end
 .
 
@@ -252,7 +251,8 @@ Definition stx_eq store v1 v2 :=
   | value_false, value_false => result_some value_true
   | value_number n1, value_number n2 => result_some (bool_to_value (_number_eq_bool n1 n2))
   | value_object ptr1, value_object ptr2 => result_some (bool_to_value (beq_nat ptr1 ptr2))
-  | value_closure id1 _ _ _, value_closure id2 _ _ _ => result_some (bool_to_value (beq_nat id1 id2))
+  | value_closure (closure_intro id1 _ _ _ _), value_closure (closure_intro id2 _ _ _ _) => 
+    result_some (bool_to_value (beq_nat id1 id2))
   | _, _ => result_some value_false
   end
 .
@@ -266,7 +266,8 @@ Definition abs_eq store v1 v2 :=
   | value_false, value_false => result_some value_true
   | value_number n1, value_number n2 => result_some (bool_to_value (_number_eq_bool n1 n2))
   | value_object ptr1, value_object ptr2 => result_some (bool_to_value (beq_nat ptr1 ptr2))
-  | value_closure id1 _ _ _, value_closure id2 _ _ _ => result_some (bool_to_value (beq_nat id1 id2))
+  | value_closure (closure_intro id1 _ _ _ _), value_closure (closure_intro id2 _ _ _ _) => 
+    result_some (bool_to_value (beq_nat id1 id2))
   | value_null, value_undefined => result_some value_true
   | value_undefined, value_null => result_some value_true
   | value_number n, value_string s
