LambdaS5/coq/LjsSyntaxAux.v
@@ -1,0 +1,16 @@
+Set Implicit Arguments.
+Require Import Utils.
+Require Import LjsShared.
+Require Export LjsSyntax.
+
+Implicit Type st : store.
+Implicit Type e : expr.
+Implicit Type v : value.
+Implicit Type c : ctx.
+Implicit Type ptr : object_ptr.
+Implicit Type obj : object.
+
+Global Instance value_inhab : Inhab value.
+Proof.
+    intros. apply (prove_Inhab value_undefined).
+Qed.
